code/hmac/Hacl.HMAC.fst
@@ -43,7 +43,7 @@ let xor_bytes_inplace a b len =
 
 // we rely on the output being zero-initialized for the correctness of padding
 inline_for_extraction noextract
-let wrap_key_st (a: const_alg) =
+let wrap_key_st (a: fixed_len_alg) =
   output: B.buffer uint8 { B.length output == block_length a } ->
   key: B.buffer uint8 {B.length key `less_than_max_input_length` a /\ B.disjoint output key} ->
   len: UInt32.t {v len = B.length key} ->
@@ -57,14 +57,14 @@ let wrap_key_st (a: const_alg) =
 
 /// This one is only to avoid a warning about a pattern that is not encoding properly.
 inline_for_extraction
-let helper_smtpat (a: const_alg) (len: uint32_t{ v len `less_than_max_input_length` a }):
+let helper_smtpat (a: fixed_len_alg) (len: uint32_t{ v len `less_than_max_input_length` a }):
   x:uint32_t { x `FStar.UInt32.lte` D.block_len a } =
   if len `FStar.UInt32.lte` D.block_len a then len else D.hash_len a
 
 #set-options "--z3rlimit 40"
 
 inline_for_extraction noextract
-let mk_wrap_key (a: const_alg) (hash: D.hash_st a): wrap_key_st a =
+let mk_wrap_key (a: fixed_len_alg) (hash: D.hash_st a): wrap_key_st a =
 fun output key len ->
   //[@inline_let] //18-08-02 does *not* prevents unused-but-set-variable warning in C
   let i = helper_smtpat a len in
@@ -92,7 +92,7 @@ fun output key len ->
   end
 
 inline_for_extraction noextract
-let block_len_as_len (a: const_alg { not (is_keccak a) }):
+let block_len_as_len (a: fixed_len_alg { not (is_keccak a) }):
   Tot (l:len_t a { len_v a l = block_length a })
 =
   let open FStar.Int.Cast.Full in
@@ -108,7 +108,7 @@ let block_len_as_len (a: const_alg { not (is_keccak a) }):
 /// necessarily disjoint).
 inline_for_extraction noextract
 val part2:
-  a: const_alg ->
+  a: fixed_len_alg ->
   m : D.m_spec a ->
   init: D.init_st (|a, m|) ->
   update_multi: D.update_multi_st (|a, m|) ->
@@ -148,7 +148,7 @@ let zero_to_len (a:hash_alg) : (if is_keccak a then unit else (x:len_t a { len_v
 
 inline_for_extraction noextract
 val part2_update_empty:
-  a: const_alg ->
+  a: fixed_len_alg ->
   m : D.m_spec a ->
   init: D.init_st (|a, m|) ->
   update_multi: D.update_multi_st (|a, m|) ->
@@ -222,7 +222,7 @@ let len_add32 a prev_len input_len =
 
 inline_for_extraction noextract
 val part2_update_nonempty:
-  a: const_alg ->
+  a: fixed_len_alg ->
   m : D.m_spec a ->
   init: D.init_st (|a, m|) ->
   update_multi: D.update_multi_st (|a, m|) ->
@@ -354,7 +354,7 @@ let part2 a m init update_multi update_last finish s dst key data len =
 /// output buffer.
 inline_for_extraction noextract
 val part1:
-  a: const_alg ->
+  a: fixed_len_alg ->
   m : D.m_spec a ->
   init: D.init_st (|a, m|) ->
   update_multi: D.update_multi_st (|a, m|) ->
@@ -382,7 +382,7 @@ let part1 a m init update_multi update_last finish s key data len =
   part2 a m init update_multi update_last finish s dst key data len
 
 let block_len_positive (a: hash_alg): Lemma (D.block_len a `FStar.UInt32.gt` 0ul) = ()
-let hash_lt_block (a: const_alg): Lemma (hash_length a < block_length a) = ()
+let hash_lt_block (a: fixed_len_alg): Lemma (hash_length a < block_length a) = ()
 
 #set-options "--z3rlimit 200"
 let mk_compute i hash alloca init update_multi update_last finish dst key key_len data data_len =
